.old/fsm.lean
@@ -1,0 +1,59 @@
+
+  structure FiniteStateMachine (α: Type) where
+    Q: Type
+    [decQ: DecidableEq Q]
+    [finQ: Fintype Q]
+    δ: Q → α → Q
+    q0: Q
+
+
+  namespace FiniteStateMachine
+
+    instance (M : FiniteStateMachine α) : DecidableEq M.Q := M.decQ
+    instance (M : FiniteStateMachine α) : Fintype M.Q   := M.finQ
+    instance (M : FiniteStateMachine α) : Inhabited M.Q := ⟨ M.q0 ⟩
+
+    instance Qalpha (M: FiniteStateMachine α): Alphabet M.Q := ⟨⟩
+
+    def scanr_step {M: FiniteStateMachine α} q a
+    | []   => [M.δ q a]
+    | qs@(q::_) => (M.δ q a :: qs)
+
+    def scanr_q {M: FiniteStateMachine α} (w: Word α) (q: M.Q): Word M.Q :=
+      w.foldr (scanr_step q) []
+
+    def scanr {M: FiniteStateMachine α} w := M.scanr_q w M.q0
+
+    def scanr_reduce {M: FiniteStateMachine α} (w: Word α): M.Q :=
+      match M.scanr w with
+      | []   => M.q0
+      | q::_ => q
+
+    @[simp, grind =]
+    lemma scanr_q_len {M: FiniteStateMachine α} (q: M.Q) (w: List α):
+      (M.scanr_q w q).length = w.length := by
+      induction w with
+      | nil => simp [scanr_q]
+      | cons a ws ih =>
+        simp [scanr_q]
+        unfold scanr_step
+        split
+        · next h =>
+          change M.scanr_q ws q = [] at h
+          rw [← ih]
+          rw [h]
+          simp
+        · next q' tail h =>
+          change M.scanr_q ws q = q' :: tail at h
+          rw [← ih]
+          rw [h]
+          simp
+
+
+    @[simp, grind =]
+    lemma scanr_len (M: FiniteStateMachine α) (w: List α): (M.scanr w).length = w.length := by
+      simp [scanr, scanr_q_len]
+
+
+
+  end FiniteStateMachine
