CellularAutomatas/all.lean
@@ -1,0 +1,5 @@
+import CellularAutomatas.defs
+import CellularAutomatas.results
+import CellularAutomatas.results_unproven
+import CellularAutomatas.proofs.common
+import CellularAutomatas.proofs.is_two_stage_of_rt_closed_and_prefix_stable
