CellularAutomatas/open_questions.lean
@@ -8,8 +8,8 @@ import Mathlib.Data.Nat.Lattice
 import Mathlib.Data.Fintype.Prod
 import CellularAutomatas.defs
 
-variable {α: Type u} [Alphabet α]
-variable {Γ: Type u} [Alphabet Γ]
+variable {α: Type} [Alphabet α]
+variable {Γ: Type} [Alphabet Γ]
 
 -- open question: is every rt_closed advice a two-stage advice?
 theorem open_question_1 (adv: Advice α Γ) (h: adv.rt_closed): adv.is_two_stage_advice := by
