CellularAutomatas/proofs/cart_transducers.lean
@@ -1,0 +1,62 @@
+import CellularAutomatas.defs
+import Mathlib.Data.List.Basic
+
+private lemma list_map_congr {α β} {f g : α → β} {l : List α} (h : ∀ x ∈ l, f x = g x) : l.map f = l.map g := by
+  induction l with
+  | nil => rfl
+  | cons a l ih =>
+  simp only [List.map_cons, List.cons.injEq]
+  constructor
+  · apply h; simp
+  · apply ih; intro x hx; apply h; simp [hx]
+
+
+lemma nextt_congr (C: CellAutomaton) (c1 c2: Config C.Q) (t: ℕ) (i: ℤ):
+    (∀ j, i - t ≤ j ∧ j ≤ i + t → c1 j = c2 j) →
+    (C.nextt c1 t) i = (C.nextt c2 t) i := by
+  induction t generalizing i c1 c2 with
+  | zero =>
+    intro h
+    simp [CellAutomaton.nextt, apply_iterated]
+    apply h
+    constructor <;> omega
+  | succ t ih =>
+    intro h
+    simp [CellAutomaton.nextt, apply_iterated]
+    -- The goal is now nextt (next c1) t i = nextt (next c2) t i
+    apply ih
+    intro j hj
+    unfold CellAutomaton.next
+    congr 1
+    · apply h
+      constructor <;> omega
+    · apply h
+      constructor <;> omega
+    · apply h
+      constructor <;> omega
+
+theorem LCellAutomaton.scan_temporal_independence [Alphabet α] (C: LCellAutomaton α) (p s: Word α):
+  (C.scan_temporal_rt (p ++ s)).take p.length = C.scan_temporal_rt p := by
+  unfold LCellAutomaton.scan_temporal_rt LCellAutomaton.scan_temporal
+  rw [← List.map_take, List.take_range, min_eq_left (by simp)]
+  apply list_map_congr
+  intro t ht
+  rw [List.mem_range] at ht
+  apply nextt_congr
+  intro j hj
+  unfold LCellAutomaton.embed_word
+  split_ifs with h1 h2
+  · congr 1
+    unfold Word.get'
+    simp only [List.get_eq_getElem]
+    apply List.getElem_append_left
+  · exfalso; unfold Word.range at *; simp at *; omega
+  · exfalso; unfold Word.range at *; simp at *; omega
+  · rfl
+
+theorem CArtTransducer.scan_temporal_independence [Alphabet α] [Alphabet Γ] (C: CArtTransducer α Γ) (p s: Word α):
+  (C.advice.f (p ++ s)).take p.length = C.advice.f p := by
+  unfold CArtTransducer.advice
+  simp
+  rw [←List.map_take]
+  rw [LCellAutomaton.scan_temporal_independence]
